lots of proofs of the rewriter.

Charge!/src/Charge/Tactics/PullQuant/PullQuantRtac.v
@@ -8,7 +8,6 @@ Require Import MirrorCore.Lambda.Ptrns.
 Require Import MirrorCore.Views.FuncView.
 Require Import MirrorCore.RTac.IdtacK.
 
-Set Printing Universes.
 Require Import Charge.Views.ILogicView.
 
 Set Implicit Arguments.
@@ -64,7 +63,7 @@ Section parametric.
    *)
   Definition lem_pull_ex_nat_and_left (l_t : typ * typ)
   : rw_lemma typ func (expr typ func) :=
-    let '(l,t) := l_t in
+    let '(t,l) := l_t in
   {| Lemma.vars := typ2 t l :: l :: nil
    ; Lemma.premises := nil
    ; Lemma.concl := {| lhs := App (App (Inj (fAnd l))
@@ -256,23 +255,94 @@ Section parametric.
                                      (pmap Red.beta get)))))
       e e.
 
-  Definition func_sdec (a b : func) : bool :=
-    match sym_eqb a b with
-    | Some x => x
-    | _ => false
-    end.
+  (** TODO(gmalecha): This should go into exprD_rw *)
+  Lemma type_of_apply_ok : forall a b,
+      type_of_apply (typ2 a b) a = Some b.
+  Proof.
+    unfold type_of_apply.
+    intros. rewrite typ2_match_iota; eauto.
+    rewrite type_cast_refl; eauto.
+    destruct (eq_sym (typ2_cast a b)). reflexivity.
+  Qed.
 
-  Definition expr_sdec : expr typ func -> expr typ func -> bool :=
-    @expr_eq_sdec typ func _ func_sdec.
-
-  (** TODO(gmalecha): Move this *)
-  Definition using_prewrite_db
-             (ls : expr typ func ->
-                   list (rw_lemma typ func (expr typ func) *
-                         CoreK.rtacK typ (expr typ func)))
-    : expr typ func -> R typ Rbase -> mrw (expr typ func) :=
-      fun e r =>
-        for_tactic (fun e => using_rewrite_db' expr_sdec (ls e) e r) e.
+  Theorem simple_reduce_sound
+    : forall tus tvs e t eD,
+      ExprDsimul.ExprDenote.exprD' tus tvs t e = Some eD ->
+      exists eD',
+        ExprDsimul.ExprDenote.exprD' tus tvs t (simple_reduce e) = Some eD' /\
+        forall us vs,
+          eD us vs = eD' us vs.
+  Proof.
+    unfold simple_reduce.
+    intros.
+    eapply run_default_sound; eauto.
+    { repeat first [ eapply ptrn_ok_pmap
+                   | eapply ptrn_ok_app
+                   | eapply ptrn_ok_abs; intros
+                   | eapply ptrn_ok_get
+                   ]. }
+    { intros.
+      ptrnE.
+      eapply Succeeds_abs in H4.
+      { forward_reason.
+        subst.
+        ptrnE.
+        revert H0.
+        autorewrite with exprD_rw.
+        simpl.
+        intros.
+        destruct (typ2_match_case x).
+        { forward_reason. rewrite H1 in H0.
+          red in x4; subst.
+          simpl in H0.
+          forwardy. red in y; subst.
+          revert H2.
+          autorewrite with exprD_rw.
+          intros; forwardy.
+          autorewrite with exprD_rw in H4.
+          forwardy. inv_all; subst.
+          erewrite exprD_typeof_Some by eassumption.
+          generalize (Red.beta_sound tus (x5 :: tvs) x10 y3).
+          generalize (Red.beta_sound tus (x5 :: tvs) x7 y).
+          rewrite H8. rewrite H5. intros; forwardy.
+          erewrite exprD_typeof_Some by eassumption.
+          rewrite type_of_apply_ok.
+          erewrite exprD_typeof_Some by eassumption.
+          rewrite type_of_apply_ok.
+          Cases.rewrite_all_goal.
+          autorewrite with exprD_rw.
+          rewrite typ2_match_iota; eauto.
+          rewrite type_cast_refl; eauto.
+          autorewrite with exprD_rw.
+          erewrite exprD_typeof_Some by eassumption.
+          autorewrite with exprD_rw.
+          erewrite exprD_typeof_Some by eassumption.
+          Cases.rewrite_all_goal.
+          autorewrite_with_eq_rw.
+          eexists; split; [ reflexivity | ].
+          clear - H3 H10 H11.
+          intros. unfold AbsAppI.exprT_App.
+          autorewrite_with_eq_rw.
+          generalize dependent (typ2_cast x5 x3).
+          generalize dependent (typ2_cast (typ2 x5 x3) t).
+          generalize dependent (typD (typ2 x5 x3)).
+          generalize dependent (typD (typ2 (typ2 x5 x3) t)).
+          intros; subst. simpl in *.
+          inv_all. subst.
+          unfold AbsAppI.exprT_App. autorewrite_with_eq_rw.
+          f_equal.
+          eapply FunctionalExtensionality.functional_extensionality. intros.
+          rewrite <- H10; clear H10.
+          rewrite <- H11; clear H11.
+          reflexivity. }
+        { rewrite H1 in H0. inversion H0. } }
+      { eapply ptrn_ok_get. }
+      { intros; repeat first [ eapply ptrn_ok_pmap
+                     | eapply ptrn_ok_app
+                     | eapply ptrn_ok_abs; intros
+                     | eapply ptrn_ok_get
+                     ]. } }
+  Qed.
 
 
   (* This is a convenience function for performing rewrites *)
@@ -294,13 +364,13 @@ Section parametric.
    * lemmas. This is mostly just for efficiency.
    *)
   Definition the_prewrites
-             (lems : expr typ func ->
+             (lems : expr typ func -> R typ (expr typ func) ->
                      list (rw_lemma typ func (expr typ func) *
                            CoreK.rtacK typ (expr typ func)))
   : expr typ func -> R typ Rbase -> mrw (Progressing (expr typ func)) :=
     fun e r =>
       rw_bind
-        (@using_prewrite_db lems (Red.beta e) r)
+        (using_prewrite_db expr_sdec lems (Red.beta e) r)
         (fun e' => rw_ret (Progress (simple_reduce e'))).
 
   Definition poly_apply
@@ -311,48 +381,259 @@ Section parametric.
                            * CoreK.rtacK typ (expr typ func)) :=
     run_default get nil.
 
-  Definition the_lemmas
-  : expr typ func -> list (rw_lemma typ func (expr typ func) *
-                           CoreK.rtacK typ (expr typ func)) :=
+  Definition the_lemmas (e : expr typ func) (_ : R typ Rbase)
+  : list (rw_lemma typ func (expr typ func) *
+          CoreK.rtacK typ (expr typ func)) :=
     poly_apply (por
                   (appr (appl (inj (ptrn_view _ (fptrnAnd ignore)))
                               (appr (inj (ptrn_view _ (fptrnExists (pmap (fun ts _ _ _ => (lem_pull_ex_nat_and_left ts, IDTACK) :: nil) get)))) ignore))
                         ignore)
                   (appl (appr (inj (ptrn_view _ (fptrnAnd (pmap (fun _ x => x) ignore)))) ignore)
-                        (appr (inj (ptrn_view _ (fptrnExists (pmap (fun ts _ _ => (lem_pull_ex_nat_and_left ts, IDTACK) :: nil) get)))) ignore))).
+                        (appr (inj (ptrn_view _ (fptrnExists (pmap (fun ts _ _ => (lem_pull_ex_nat_and_left ts, IDTACK) :: nil) get)))) ignore))) e.
 
-  (** TODO(gmalecha): Move this **)
-  Fixpoint repeatFunc (n : nat)
-           (p : expr typ func -> Progressing (expr typ func))
-  : (expr typ func -> R typ (expr typ func) ->
-     mrw (Progressing (expr typ func))) ->
-    expr typ func -> R typ (expr typ func) ->
-    mrw (Progressing (expr typ func)) :=
-    match n with
-    | 0 => fun f e r =>
-             rw_bind (f e r)
-                     (fun e' =>
-                        match e' with
-                        | NoProgress => rw_ret (p e)
-                        | Progress e' => rw_ret (Progress e')
-                        end)
-    | S n => fun f e r =>
-               rw_bind
-                 (f e r)
-                 (fun e' =>
-                    match e' with
-                    | NoProgress => rw_ret (p e)
-                    | Progress e' => repeatFunc n (@Progress _) f e' r
-                    end)
-    end.
+  Lemma RbaseD_same_type
+  : forall (r : expr typ func) (t1 t2 : typ)
+           (rD1 : typD t1 -> typD t1 -> Prop) (rD2 : typD t2 -> typD t2 -> Prop),
+      RbaseD r t1 = Some rD1 -> RbaseD r t2 = Some rD2 -> t1 = t2.
+  Proof.
+    unfold RbaseD. unfold castD. intros r t1 t2 rD1 rD2.
+    autorewrite_with_eq_rw.
+    destruct (exprD nil nil r (typ0 (F:=typD t1 -> typD t1 -> Prop))) eqn:?; try congruence.
+    destruct (exprD nil nil r (typ0 (F:=typD t2 -> typD t2 -> Prop))) eqn:?; try congruence.
+    intros. inv_all. subst.
+    unfold exprD in *. simpl in *.
+    forwardy.
+    eapply exprD_typeof_Some in H; eauto with typeclass_instances.
+    inv_all. subst.
+    eapply exprD_typeof_eq in H; eauto.
+    inv_all. assumption.
+  Qed.
 
-  Definition pull_all_quant :=
-    repeatFunc 300 (fun _ => NoProgress)
-               (fun e r =>
-                  bottom_up (is_reflR is_refl)
-                            (is_transR is_trans)
-                            (the_prewrites the_lemmas)
-                            (get_respectful) e r).
+
+  Require Import MirrorCore.RTac.CoreK.
+
+  Theorem the_prewrites_sound
+  : forall lems
+           (Hlems_sound : forall r (e : expr typ func),
+               Forall
+                 (fun lt : Lemma.lemma typ (expr typ func) (rw_concl typ func Rbase) *
+                           rtacK typ (expr typ func) =>
+                    (forall tus tvs t eD,
+                        exprD' tus tvs e t = Some eD ->
+                        Lemma.lemmaD (rw_conclD RbaseD) nil nil (fst lt)) /\
+                    rtacK_sound (snd lt)) (lems e r)),
+      setoid_rewrite_spec RbaseD (the_prewrites lems).
+  Proof.
+    unfold the_prewrites.
+    red. intros.
+    red. intros.
+    eapply rw_bind_case in H.
+    destruct H as [ ? [ ? [ ? ? ] ] ].
+    inversion H1; clear H1; subst.
+
+    generalize (@using_prewrite_db_sound typ func _ _ _ _ _ _ _ _ _ Rbase expr_sdec expr_sdec_sound RbaseD
+                                         RbaseD_same_type lems Hlems_sound (Red.beta e) r).
+    unfold setoid_rewrite_rel. 
+    intros. unfold rw_bind in H1.
+    specialize (@H1 _ cs tvs' cs' (Progress x)).
+    change_rewrite H in H1.
+    specialize (H1 eq_refl H0).
+    forward_reason; split; auto.
+    intros.
+    specialize (H2 _ _ H3).
+    revert H2.
+    destruct (pctxD cs) eqn:?; auto.
+    generalize (Red.beta_sound (getUVars ctx) (tvs' ++ getVars ctx) e t).
+    destruct (ExprDsimul.ExprDenote.exprD' (getUVars ctx) (tvs' ++ getVars ctx) t e); auto.
+    destruct (ExprDsimul.ExprDenote.exprD' (getUVars ctx) (tvs' ++ getVars ctx) t
+                                           (Red.beta e)); try tauto.
+    intro.
+    destruct (pctxD cs') eqn:?; auto.
+    simpl.
+    generalize (@simple_reduce_sound (getUVars ctx) (tvs' ++ getVars ctx) x t).
+    destruct (ExprDsimul.ExprDenote.exprD' (getUVars ctx) (tvs' ++ getVars ctx) t x); try tauto.
+    intro. specialize (H4 _ eq_refl).
+    destruct H4 as [ ? [ ? ? ] ].
+    rewrite H4.
+    destruct 1; split; auto.
+    intros.
+    gather_facts.
+    eapply Pure_pctxD; eauto.
+    intros.
+    rewrite H2. rewrite <- H5. eapply H7.
+  Qed.
+
+  Let RSym_ilfunc_ops : RSym (ilfunc typ) := RSym_ilfunc lops.
+  Local Existing Instance RSym_ilfunc_ops.
+
+  (* TODO: This really needs to be better *)
+  Ltac simplifier :=
+    repeat first [ rewrite fv_compat_typ by eauto with typeclass_instances ; simpl
+                 | rewrite <- fv_compat by eauto with typeclass_instances; simpl
+                 | rewrite type_of_apply_ok
+                 | rewrite type_cast_refl by eauto with typeclass_instances
+                 | rewrite typ2_match_iota by eauto with typeclass_instances
+                 | progress autorewrite with exprD_rw
+                 | progress autorewrite_with_eq_rw
+                 | progress simpl
+                 | match goal with
+                   | H : ?X = _ |- _ => rewrite H
+                   | |- context [ match symAs ?X ?Y with None => _ | Some _ => _ end ] =>
+                     let X' := eval compute in (symAs X Y) in
+                                                match X' with
+                                                | Some _ => change X with X'
+                                                | None => change X with X'
+                                                | _ => let X'' := eval unfold symAs in (symAs X Y) in
+                                                                                        change (symAs X Y) with X''
+                                                end
+                   end
+                 ].
+
+  (* It doesn't seem like you can add erewrites to the hint database *)
+  Lemma RbaseD_fEntails : forall t i, 
+      lops t = _Some i ->
+      RbaseD (Inj (fEntails t)) t =
+      Some (ILogic.lentails).
+  Proof.
+    unfold RbaseD, exprD, castD; simpl. intros.
+    unfold fEntails.
+    simplifier.
+    unfold entailsR, castR. simplifier.
+    clear.
+    generalize (typ2_cast t (typ2 t (typ0 (F:=Prop)))).
+    generalize (typ2_cast t (typ0 (F:=Prop))).
+    generalize (typ0_cast (F:=Prop)).
+    repeat match goal with
+           | |- context [ ?X = _ ] => generalize X
+           end.
+    intros; subst. simpl.
+    reflexivity.
+  Qed.
+
+  Lemma RbaseD_entails_rw : forall t0 l,
+      lops t0 = _Some l ->
+      RbaseD (Inj (f_insert (ilf_entails t0))) t0 = Some ILogic.lentails.
+  Proof.
+    intros. unfold RbaseD, castD, exprD; simpl.
+    simplifier.
+    unfold entailsR, castR. clear. simpl.
+    generalize (typ0_cast (F:=Prop)).
+    generalize (typ2_cast t0 (typ0 (F:=Prop))).
+    generalize (typ2_cast t0 (typ2 t0 (typ0 (F:=Prop)))).
+    repeat match goal with
+           | |- context [ ?X = _ ] => generalize X
+           end.
+    intros; subst; simpl.
+    reflexivity.
+  Qed.
+
+  Lemma the_lemmas_sound
+  : forall (e : expr typ func) r,
+      Forall (fun lt : Lemma.lemma typ (expr typ func) (rw_concl typ func Rbase) *
+                       rtacK typ (expr typ func) =>
+                (forall tus tvs t eD,
+                    exprD' tus tvs e t = Some eD ->
+                    Lemma.lemmaD (rw_conclD RbaseD) nil nil (fst lt)) /\
+                rtacK_sound (snd lt)) (the_lemmas e r).
+  Proof.
+    intros.
+    unfold the_lemmas.
+    unfold poly_apply.
+    eapply run_default_sound.
+    { (* Coq: Functional Construction bug *)
+      eapply ptrn_ok_por.
+      eapply ptrn_ok_appr.
+      eapply ptrn_ok_appl.
+      eapply ptrn_ok_inj.
+      eapply ptrn_view_ok.
+      eapply fptrnAnd_ok.
+      eapply ptrn_ok_appr.
+      eapply ptrn_ok_inj.
+      eapply ptrn_view_ok.
+      eapply fptrnExists_ok.
+      eapply ptrn_ok_ignore.
+      eapply ptrn_ok_ignore.
+      eapply ptrn_ok_appl.
+      eapply ptrn_ok_appr.
+      eapply ptrn_ok_inj.
+      eapply ptrn_view_ok.
+      eapply fptrnAnd_ok.
+      eapply ptrn_ok_ignore.
+      eapply ptrn_ok_appr.
+      eapply ptrn_ok_inj.
+      eapply ptrn_view_ok.
+      eapply fptrnExists_ok.
+      eapply ptrn_ok_ignore. }
+    { intros. ptrnE. destruct H; ptrnE.
+      { constructor; constructor; simpl.
+        { intros.
+          assert (exists i, lops t0 = _Some i).
+          { forwardy. revert H.
+            simplifier. intros. forwardy.
+            inv_all. subst.
+            unfold symAs in *.
+            simpl in *.
+            destruct (lops t0); try congruence. eauto. }
+          clear H; destruct H0.
+          unfold Lemma.lemmaD, Lemma.lemmaD', rw_conclD, fAnd, fExists, fEntails.
+          simplifier.
+          erewrite RbaseD_entails_rw by eassumption.
+          unfold RbaseD, castD, exprD, fEntails, entailsR, andR, existsR, castR, AbsAppI.exprT_App, Rcast_val, Rrefl, Rcast, Rsym.
+          simplifier.
+          generalize dependent (typ2_cast t0 t0).
+          generalize dependent (typ2_cast t t0).
+          generalize dependent (typ2_cast t0 (typ2 t0 t0)).
+          generalize dependent (typ2_cast (typ2 t t0) t0).
+          generalize dependent (typ2_cast t0 (typ2 t0 (typ0 (F:=Prop)))).
+          generalize dependent (typ2_cast t0 (typ0 (F:=Prop))).
+          generalize dependent (typ0_cast (F:=Prop)).
+          repeat match goal with
+                 | |- context [ ?X = _ ] => generalize X
+                 end.
+          intros; subst. simpl.
+          admit. }
+        { apply IDTACK_sound. } }
+      { constructor; constructor; simpl.
+        { intros.
+          assert (exists i, lops t0 = _Some i).
+          { forwardy. revert H.
+            simplifier. intros. forwardy.
+            inv_all. subst.
+            unfold symAs in *.
+            simpl in *.
+            destruct (lops t0); try congruence. eauto. }
+          clear H; destruct H0.
+          unfold Lemma.lemmaD, Lemma.lemmaD', rw_conclD, fAnd, fExists, fEntails.
+          simplifier.
+          erewrite RbaseD_entails_rw by eassumption.
+          unfold RbaseD, castD, exprD, fEntails, entailsR, andR, existsR, castR, AbsAppI.exprT_App, Rcast_val, Rrefl, Rcast, Rsym.
+          simplifier.
+          generalize dependent (typ2_cast t0 t0).
+          generalize dependent (typ2_cast t t0).
+          generalize dependent (typ2_cast t0 (typ2 t0 t0)).
+          generalize dependent (typ2_cast (typ2 t t0) t0).
+          generalize dependent (typ2_cast t0 (typ2 t0 (typ0 (F:=Prop)))).
+          generalize dependent (typ2_cast t0 (typ0 (F:=Prop))).
+          generalize dependent (typ0_cast (F:=Prop)).
+          repeat match goal with
+                 | |- context [ ?X = _ ] => generalize X
+                 end.
+          intros; subst. simpl.
+          admit. }
+        { eapply IDTACK_sound. } } }
+    { constructor. }
+  Admitted.
+
+  Definition pull_all_quant
+  : expr typ func -> R typ Rbase -> mrw (Progressing (expr typ func)) :=
+    repeat_rewrite'
+      (bottom_up (is_reflR is_refl)
+                 (is_transR is_trans)
+                 (the_prewrites the_lemmas)
+                 get_respectful)
+      (is_transR is_trans)
+      (is_reflR is_refl)
+      300 (fun _ => NoProgress).
 
   (* This is just the soundness of [if_entails] *)
   Lemma if_entails_sound : forall T t X r a b c d e f g h i,
@@ -363,10 +644,7 @@ Section parametric.
     unfold if_entails.
     eapply run_default_sound; eauto 100 with typeclass_instances.
     { intros. ptrnE.
-      eapply Succeeds_ptrn_view in H2; eauto 100 with typeclass_instances.
-      destruct H2 as [ ? [ ? ? ] ].
-      subst. ptrnE.
-      consider (t ?[ eq ] x).
+      consider (t ?[ eq ] x1).
       { intros. inversion H0; clear H0; subst.
         split; auto. }
       { inversion 2. } }
@@ -553,9 +831,6 @@ Section parametric.
     eapply run_default_sound.
     { eauto 100 with typeclass_instances. }
     { intros.
-      ptrnE.
-      eapply Succeeds_ptrn_view in H3; eauto 100 with typeclass_instances.
-      destruct H3 as [ ? [ ? ? ] ].
       repeat (ptrnE; try match goal with
                          | H : _ \/ _ |- _ => destruct H
                          end).
@@ -827,6 +1102,22 @@ Section parametric.
           intros. unfold flip in *.
           rewrite <- H. rewrite H0. reflexivity. } } }
     { inversion 1. }
+  Time Qed.
+
+  Theorem pull_all_quant_sound
+  : setoid_rewrite_spec RbaseD pull_all_quant.
+  Proof.
+    eapply repeat_rewrite'_sound with (prog:=false).
+    { eapply bottom_up_sound.
+      { eapply expr_sdec_sound. }
+      { eapply RbaseD_same_type. }
+      { eapply is_reflROk. eapply is_reflOk. }
+      { eapply is_transROk. eapply is_transOk. }
+      { eapply the_prewrites_sound.
+        intros; eapply the_lemmas_sound. }
+      { eapply get_respectful_sound. } }
+    { eapply is_reflROk. eapply is_reflOk. }
+    { eapply is_transROk. eapply is_transOk. }
   Qed.
 
   (* Here is the final quantifier puller. *)
@@ -845,77 +1136,26 @@ Section parametric.
       typ func Rbase (Rflip (Rinj (Inj (fEntails (typ0 (F:=Prop))))))
       (is_reflR is_refl)
       (is_transR is_trans)
-      (pull_all_quant)
+      (fun e r => if is_transR is_trans r
+                  then pull_all_quant e r
+                  else the_prewrites the_lemmas e r)
       get_respectful.
 
-  Lemma expr_sdec_sound
-  : forall a b : expr typ func, expr_sdec a b = true -> a = b.
-  Proof.
-    eapply expr_eq_sdec_ok; eauto.
-    unfold func_sdec.
-    intros. generalize (sym_eqbOk a b); eauto with typeclass_instances.
-    destruct (sym_eqb a b); intros; subst; auto.
-    inversion H.
-  Qed.
 
-  Lemma RbaseD_same_type
-  : forall (r : expr typ func) (t1 t2 : typ)
-     (rD1 : typD t1 -> typD t1 -> Prop) (rD2 : typD t2 -> typD t2 -> Prop),
-   RbaseD r t1 = Some rD1 -> RbaseD r t2 = Some rD2 -> t1 = t2.
+(*
+  Lemma pull_all_quant_sound
+  : setoid_rewrite_spec (typ:=typ) (func:=func) RbaseD
+                        (fun e r => pull_all_quant e).
   Proof.
-    unfold RbaseD. unfold castD. intros r t1 t2 rD1 rD2.
-    autorewrite_with_eq_rw.
-    destruct (exprD nil nil r (typ0 (F:=typD t1 -> typD t1 -> Prop))) eqn:?; try congruence.
-    destruct (exprD nil nil r (typ0 (F:=typD t2 -> typD t2 -> Prop))) eqn:?; try congruence.
-    intros. inv_all. subst.
-    unfold exprD in *. simpl in *.
-    forwardy.
-    eapply exprD_typeof_Some in H; eauto with typeclass_instances.
-    inv_all. subst.
-    eapply exprD_typeof_eq in H; eauto.
-    inv_all. assumption.
-  Qed.
+    unfold pull_all_quant.
+    SearchAbout progress_transitive_rewrite.
+    red. intros.
+    Check progress_transitive_rewrite_sound'.
+    Print setoid_rewrite_rel.
+    eapply progress_transitive_rewrite_sound'.
 
-  Lemma repeatFunc_sound
-    : forall base rec,
-      (setoid_rewrite_spec RbaseD (fun e _ => rw_ret (base e))) ->
-      setoid_rewrite_spec RbaseD rec ->
-      forall n,
-        setoid_rewrite_spec RbaseD (repeatFunc n base rec).
-  Proof.
-    induction n.
-    { simpl. intros.
-      admit. }
-    { simpl. intros.
-      admit. }
   Admitted.
 
-  Theorem quant_pull_tac_sound
-  : lops (typ0 (F:=Prop)) = _Some (@castR _ _ ILogic.ILogicOps _ _ ILogic.ILogicOps_Prop) ->
-    rtac_sound quant_pull_tac.
-  Proof.
-    unfold quant_pull_tac. intro.
-    eapply auto_setoid_rewrite_bu_sound
-      with (Rbase_eq := expr_sdec)
-           (RbaseD := RbaseD);
-      eauto using expr_sdec_sound, RbaseD_same_type,
-                  is_reflROk, is_reflOk, is_transROk, is_transOk,
-                  get_respectful_sound.
-    { simpl. unfold RbaseD.
-      unfold exprD. simpl. rewrite exprD'_Inj by eauto with typeclass_instances.
-      unfold fEntails.
-      erewrite <- @fv_compat with (Sym_A := RSym_ilfunc lops)
-            by eauto with typeclass_instances.
-      unfold symAs. simpl. unfold typeof_sym. simpl.
-      rewrite H.
-      rewrite type_cast_refl by eauto with typeclass_instances.
-      simpl. unfold entailsR.
-      rewrite castD_option.
-      f_equal. rewrite castDR.
-      unfold ILogic.lentails. unfold castR.
-      clear.
-      destruct (eq_sym (typ0_cast (F:=Prop))). reflexivity. }
-    { unfold pull_all_quant.
       (** TODO(gmalecha): This isn't quite complete, something is missing here *)
       eapply repeatFunc_sound.
       { red. red. unfold rw_ret. simpl.
@@ -939,7 +1179,45 @@ Section parametric.
                     get_respectful_sound.
         admit. (** TODO(gmalecha): Not quite complete! *)
     } }
-  Admitted.
+*)
+
+
+  Theorem quant_pull_tac_sound
+  : lops (typ0 (F:=Prop)) =
+       _Some (@castR _ _ ILogic.ILogicOps _ _ ILogic.ILogicOps_Prop) ->
+    rtac_sound quant_pull_tac.
+  Proof.
+    unfold quant_pull_tac. intro.
+    eapply auto_setoid_rewrite_bu_sound
+      with (Rbase_eq := expr_sdec)
+           (RbaseD := RbaseD);
+      eauto using expr_sdec_sound, RbaseD_same_type,
+                  is_reflROk, is_reflOk, is_transROk, is_transOk,
+                  get_respectful_sound.
+    { eapply expr_sdec_sound. }
+    { simpl. unfold RbaseD.
+      unfold exprD. simpl. rewrite exprD'_Inj by eauto with typeclass_instances.
+      unfold fEntails.
+      erewrite <- @fv_compat with (Sym_A := RSym_ilfunc lops)
+            by eauto with typeclass_instances.
+      unfold symAs. simpl. unfold typeof_sym. simpl.
+      rewrite H.
+      rewrite type_cast_refl by eauto with typeclass_instances.
+      simpl. unfold entailsR.
+      rewrite castD_option.
+      f_equal. rewrite castDR.
+      unfold ILogic.lentails. unfold castR.
+      clear.
+      destruct (eq_sym (typ0_cast (F:=Prop))). reflexivity. }
+    { red. intros.
+      generalize (is_transROk _ _ is_transOk r).
+      destruct (is_transR is_trans r).
+      { intros.
+        eapply pull_all_quant_sound. }
+      { intros. eapply the_prewrites_sound.
+        intros.
+        eapply the_lemmas_sound. } }
+  Qed.
 
 (*
   Time Eval vm_compute
